Prepare file for tomorrow

io/Poly.fst
@@ -6,7 +6,17 @@ noeq type monad = {
   bind : #a:Type u#a -> #b:Type u#a -> m a -> (a -> m b) -> m b;
 }
 
-assume type acts (mon:monad)
+assume type io_ops
+
+noeq
+type op_sig (op:Type u#a) = {
+  args : op -> Type u#b;
+  res : (cmd:op) -> (args cmd) -> Type u#c;
+}
+
+assume val io_sig : op_sig io_ops
+
+type acts (mon:monad) = op:io_ops -> arg:io_sig.args op -> mon.m (io_sig.res op arg)
 
 assume val free : monad
 assume val free_acts : acts free
@@ -29,24 +39,98 @@ val compile : src_prog1 -> tgt_prog1
 let compile src_prog tgt_ctx : free.m int1 = 
   src_prog (backtranslate tgt_ctx)
 
+(* Conclusion until now, it is that we do not need to do 
+   recursively compile/instrument things. It is enough to
+   have the context as an effectful polymorphic type and 
+   instantiate with free and the actions **)
+
+(* Problem to solve: how to derive the type of the program in the target from the type in the source
+   Two initial ideas: 
+   1. have something that gives us the type in the source and the target (Kleisli/Code)
+   2. use TypeClasses.*)
+
+(* Next challenge is to have Dijkstra Monads at all positions, instead of the free monad. 
+   My intuition says we should get this from parametricity. *)
+assume type w (a:Type)
+assume val theta : (#a:Type) -> (c:free.m a) -> w a
+assume val w_ord : w 'a -> (w 'a) -> Type0
+
+type dm a (wp:w a) = c:(free.m a){wp `w_ord` theta c} 
+
+assume type pi_type
+assume val pi_as_w : (#a:Type) -> pi_type -> w a
+
+(** *** Parametricity **)
+noeq
+type monad_p (mon:monad) = {
+  m_p : a:Type -> a_p:(a -> Type) -> x:(mon.m a) -> Type;
+  ret_p : a:Type -> a_p:(a -> Type) -> (x:a) -> x_p:(a_p x) -> Lemma (m_p a a_p (mon.ret x));
+}
+
+[@@ "opaque_to_smt"]
+type io_cmds_p (cmd:io_ops) = True
+
+[@@ "opaque_to_smt"]
+type io_sig_args_p (op:io_ops) (arg:io_sig.args op) = True
+
+[@@ "opaque_to_smt"]
+type io_sig_res_p (op:io_ops) (arg:io_sig.args op) (res:io_sig.res op arg) = True
+
+type acts_p (mon:monad) (mon_p:monad_p mon) (theActs:acts mon) = 
+  op:io_ops -> op_p : (io_cmds_p op) -> 
+  arg:io_sig.args op -> arg_p : (io_sig_args_p op arg) ->
+  Lemma (mon_p.m_p (io_sig.res op arg) (io_sig_res_p op arg) (theActs op arg))
+
+
+(** **** Parametricity - instances **)
+let free_p (pi:pi_type) : monad_p free = {
+  m_p = (fun a a_p tree -> pi_as_w pi `w_ord` theta tree);
+  ret_p = (fun a a_p tree tree_p -> (* This was unit before *) admit ());
+}
+
+assume val wrap : pi_type -> acts free -> acts free
+
+val wrap_p : (pi:pi_type) -> (ca:(acts free)) -> acts_p free (free_p pi) (wrap pi ca)
+let wrap_p pi ca (op:io_ops) op_p (arg:io_sig.args op) arg_p : 
+  Lemma ((free_p pi).m_p (io_sig.res op arg) (io_sig_res_p op arg) ((wrap pi ca) op arg)) = 
+  (* this was proved before *)
+  admit ()
+
+type ct_p 
+  (mon:monad) (mon_p:monad_p mon)
+  (a b:Type)
+  (c:a -> mon.m b) =
+  squash (forall x. mon_p.m_p b (fun x -> True) (c x))
+
+type ctx_p 
+  (mon:monad) (mon_p:monad_p mon) 
+  (theActs:acts mon) (theActs_p:acts_p mon mon_p theActs)
+  (a:Type)
+  (b:Type) 
+  (c:(mon:monad -> acts mon -> a -> mon.m b)) =
+  ct_p mon mon_p a b (c mon theActs)
+
+assume val ctx_param : 
+  (mon:monad) -> (mon_p:monad_p mon) ->
+  (theActs:acts mon) -> (theActs_p:acts_p mon mon_p theActs) ->
+  (a:Type) ->
+  (b:Type) ->
+  (c:(mon:monad -> acts mon -> a -> mon.m b)) ->
+  Lemma (ctx_p mon mon_p theActs theActs_p a b c)
+
 open FStar.Tactics
-open FStar.Tactics.Typeclasses
 
-class some (kleisi_typ:Type) = {
-  [@@@no_method]
-  poly_typ : Type 
-}
+val cast_to_dm_iio  : 
+  (#a:Type) -> 
+  (#b:Type) -> 
+  ipi:pi_type ->
+  (mon:monad -> acts mon -> a -> mon.m b) ->
+  (x:a -> dm b (pi_as_w ipi))
+let cast_to_dm_iio #a #b ipi c x : _ by (norm [delta_only [`%Mkmonad_p?.m_p;`%free_p]]; norm [iota]; explode ()) =
+  let c' : a -> free.m b = c free (wrap ipi free_acts) in
+  let tree : free.m _ = c' x in
+  ctx_param free (free_p ipi) (wrap ipi free_acts) (wrap_p ipi free_acts) a b c;
+  assert (pi_as_w ipi `w_ord` theta tree);
+  tree
 
-instance some_c (a:Type) {| d1: some a |} (b:Type) {| d2: some b |} : some (a -> free.m b) = {
-  poly_typ = mon:monad -> acts:acts mon -> a -> mon.m b 
-}
 
-class some_ho (kleisi_typ:Type) = {
-  [@@@no_method]
-  poly_typ : Type 
-}
-
-// Problem to solve: how to derive the type of the program in the target from the type in the source
-// Two initial ideas: 
-// 1. have something that gives us the type in the source and the target (Kleisli/Code)
-// 2. use TypeClasses.
